Parsing/Ground_PDDL_Parsing.thy
@@ -1,7 +1,6 @@
 theory Ground_PDDL_Parsing
   imports Temporal_AI_Planning_Languages_Semantics.TEMPORAL_PDDL_Semantics
           Parsing.JSON_Parsing
-          Temporal_Planning_Base.Base
           Temporal_Planning_Base.Error_List_Monad_Add
 begin
 
@@ -23,10 +22,10 @@ definition [consuming]:
   "middle l m r \<equiv> l *-- m --* r"
 
 definition [consuming]:
-  "paren_open \<equiv> token (exactly ''('')"
+  "paren_open \<equiv> (exactly ''('') \<parallel> (token (exactly ''(''))"
 
 definition [consuming]:
-  "paren_close \<equiv> token (exactly '')'')"
+  "paren_close \<equiv> (exactly '')'') \<parallel> (token (exactly '')''))"
 
 definition [consuming]:
   "parens p \<equiv> middle paren_open p paren_close"
@@ -43,7 +42,8 @@ definition
 definition 
   "pddl_reserved_keywords \<equiv> set pddl_requirement_keywords \<union> {
       ''define'', ''domain'', '':requirements'', '':predicates'', '':functions'',
-      '':types'', '':constants'', '':action'', '':parameters'', '':precondition'', '':effect'', 
+      '':types'', '':constants'', '':action'', '':durative-action'', '':parameters'', 
+      '':precondition'', '':condition'', '':duration'', '':effect'', 
       '':invariant'', '':name'', '':vars'', '':set-constraint'',
       ''problem'', '':domain'', '':init'', '':objects'', '':goal'', '':metric'', ''maximize'', ''minimize'',              
       ''='', ''+'', ''-'', ''/'', ''*'', ''<'', ''>'', ''<='', ''>='', ''.'', ''and'', ''or'', ''imply'', ''not'', ''forall'', ''exists'', ''when'',
@@ -51,21 +51,48 @@ definition
       ''number'', ''undefined'', ''total-cost'', ''object'',
       ''at'', ''start'', ''end'', ''over'', ''all'', ''?duration''}" 
 
+(* 
 definition
   "non_white_space \<equiv> do {
     x \<leftarrow> get;
     if x \<notin> (set char_wspace)
     then return x
     else err_expecting (shows ''non-whitespace character'')
+  }" *)
+
+definition
+  "lx_dash_underscore \<equiv> do {
+    x \<leftarrow> get;
+    if x \<in> {CHR ''-'', CHR ''_''}
+    then return x
+    else err_expecting (shows ''Neither dash (-) nor underscore (_)'')
   }"
 
 definition             
-  "pddl_token \<equiv> repeat1 non_white_space"
+  "pddl_token \<equiv> repeat1 (lx_alphanum \<parallel> lx_dash_underscore)"
 
+definition
+  "lx_not_whitespace_nor_parens \<equiv> do {
+    x \<leftarrow> get;
+    if x \<notin> {CHR ''('', CHR '')'', CHR ''['', CHR '']'', CHR ''{'', CHR ''}''}
+    then (
+      if x \<notin> (set char_wspace)
+      then return x
+      else err_expecting (shows ''non-whitespace character'')
+    )else err_expecting (shows ''Brackets encountered'')
+  }"
+
+definition 
+  "pddl_word \<equiv> repeat1 lx_not_whitespace_nor_parens"
+
+definition             
+  "pddl_keyword_token \<equiv> 
+    ((exactly '':'') -- pddl_word) with (uncurry (@))
+    \<parallel> pddl_word"
 
 definition
   "pddl_keyword v \<equiv> do {
-    w \<leftarrow> token pddl_token;
+    w \<leftarrow> token pddl_keyword_token;
     _ \<leftarrow> if (v \<notin> pddl_reserved_keywords) 
          then error (shows ''Invalid keyword parser: \"'' o shows v o shows ''\" is not a keyword'') 
          else return ();
@@ -82,6 +109,7 @@ definition
     else err_expecting (shows ''identifier'')
   }"
 
+
 definition 
   "pddl_domain_head \<equiv> parens (pddl_keyword ''domain'' *-- pddl_identifier)"
 
@@ -92,62 +120,55 @@ abbreviation str_to_pred::"string \<Rightarrow> object atom" where
   "str_to_pred x \<equiv> predAtm (Pred x) []"
 
 definition 
-  "pddl_predicate \<equiv> pddl_identifier with str_to_pred"
+  "pddl_predicate \<equiv> opt_parens (pddl_identifier with str_to_pred)"
 
 definition 
   "pddl_single_requirement \<equiv> 
     pddl_requirement_keywords
     |> (map pddl_keyword)
-    |> alt_list
-    |> token"
+    |> alt_list"
 
 definition
   "pddl_requirements \<equiv> parens (pddl_keyword '':requirements'' *-- repeat pddl_single_requirement)"
 
 definition
-  "pddl_predicates \<equiv> parens (pddl_keyword '':predicates'' *-- repeat (opt_parens pddl_predicate))"
+  "pddl_predicates \<equiv> parens (pddl_keyword '':predicates'' *-- repeat pddl_predicate)"
 
 definition pddl_action_params::"(char, variable list) parser" where
-  "pddl_action_params \<equiv> pddl_keyword '':parameters'' *-- parens (return [])"
+  "pddl_action_params \<equiv> pddl_keyword '':parameters'' *-- (paren_open -- paren_close) with (\<lambda>_. [])"
 
 definition
-  "pddl_and p \<equiv> pddl_keyword ''and'' *-- repeat (parens p)"
+  "pddl_and p \<equiv> parens (pddl_keyword ''and'' *-- repeat p)"
 
 definition
-  "pddl_opt_and p \<equiv> (parens (pddl_and p)) \<parallel> p with (\<lambda>x. [x])"
+  "pddl_opt_and p \<equiv> (pddl_and p) \<parallel> p with (\<lambda>x. [x])"
 
 fun fract_to_rat::"fract \<Rightarrow> rat" where
 "fract_to_rat (fract.Rat True n d) = Fract n d" |
 "fract_to_rat (fract.Rat False n d) = Fract (-n) d"
 
 definition
-  "pddl_num \<equiv> lx_rat with fract_to_rat"
+  "pddl_num \<equiv> token (lx_rat with fract_to_rat \<parallel> lx_int with of_int)"
 
 
 (* It seems that durations use inclusive bounds. *)
 definition pddl_duration_constraint::"(char, object duration_constraint) parser" where
   "pddl_duration_constraint \<equiv> 
-  ( ( (pddl_keyword ''<='' *-- return duration_op.LEQ)
-    \<parallel> (pddl_keyword ''>='' *-- return duration_op.GEQ)
-    ) --* (pddl_keyword ''?duration'')
-  ) -- pddl_num 
-  with uncurry Time_Const"
+  parens ( 
+    ( pddl_keyword ''<='' with (\<lambda>_. duration_op.LEQ)
+    \<parallel> pddl_keyword ''>='' with (\<lambda>_. duration_op.GEQ)
+    ) -- ((pddl_keyword ''?duration'') *-- pddl_num)
+  ) with uncurry Time_Const"
 
 definition 
-  "pddl_duration_constraints \<equiv> pddl_opt_and pddl_duration_constraint"
-
+  "pddl_duration_constraints \<equiv> 
+    pddl_keyword '':duration'' *-- pddl_opt_and pddl_duration_constraint"
+                 
 definition 
   "pddl_add_or_del \<equiv> 
-    (parens (pddl_keyword ''not'' *-- pddl_identifier with Inl o str_to_pred))
-    \<parallel> (pddl_identifier with (Inr o str_to_pred))"
+    (parens (pddl_keyword ''not'' *-- pddl_predicate with Pair False))
+    \<parallel> (pddl_predicate with Pair True)"
 
-fun left_sum::"('a, 'b) sum \<Rightarrow> 'a option" where
-"left_sum (Inl a) = Some a" |
-"left_sum (Inr a) = None"
-
-fun right_sum::"('a, 'b) sum \<Rightarrow> 'b option" where
-"right_sum (Inr a) = Some a" |
-"right_sum (Inl a) = None"
 
 (* fun is_left::"('a, 'b) sum \<Rightarrow> bool" where
 "is_left (Inl a) = True" |
@@ -157,12 +178,15 @@ fun is_right::"('a, 'b) sum \<Rightarrow> bool" where
 "is_right (Inr a) = False" |
 "is_right (Inl a) = True" *)
 
-definition
-  "pddl_timed_pred \<equiv> 
-    ( ((pddl_keyword ''at'' -- pddl_keyword ''start'') *-- (return At_Start))
-    \<parallel> ((pddl_keyword ''at''-- pddl_keyword ''end'') *-- (return At_End))
-    \<parallel> ((pddl_keyword ''over'' -- pddl_keyword ''all'') *-- (return Over_All))
-    ) -- pddl_opt_and pddl_predicate"
+
+definition 
+  "pddl_timed_literal l \<equiv> 
+    parens ( 
+      ( ((pddl_keyword ''at'' -- pddl_keyword ''start'') *-- (return At_Start))
+      \<parallel> ((pddl_keyword ''at''-- pddl_keyword ''end'') *-- (return At_End))
+      \<parallel> ((pddl_keyword ''over'' -- pddl_keyword ''all'') *-- (return Over_All))
+      ) -- pddl_opt_and l
+    )"
 
 definition 
   "start_filter \<equiv> (\<lambda>(a, b). if (a = At_Start) then Some b else None)"
@@ -174,37 +198,35 @@ definition
   "oa_filter \<equiv> (\<lambda>(a, b). if (a = Over_All) then Some b else None)"
 
 definition
+  "add_filter \<equiv> (\<lambda>(a, b). if (a = True) then Some b else None)"
+
+definition
+  "del_filter \<equiv> (\<lambda>(a, b). if (a = False) then Some b else None)"
+
+definition
   "pddl_conditions \<equiv> do {
-    conditions \<leftarrow> pddl_keyword '':condition'' *-- pddl_opt_and pddl_timed_pred;
-    let s_effs = conditions |> collect start_filter |> (\<lambda>xs. fold (@) xs []);
-    let e_effs = conditions |> collect end_filter |> (\<lambda>xs. fold (@) xs []);
+    conditions \<leftarrow> pddl_keyword '':condition'' *-- pddl_opt_and (pddl_timed_literal pddl_predicate);
+    let s_conds = conditions |> collect start_filter |> (\<lambda>xs. fold (@) xs []);
+    let e_conds = conditions |> collect end_filter |> (\<lambda>xs. fold (@) xs []);
     let oc = conditions |> collect oa_filter |> (\<lambda>xs. fold (@) xs []);
-    return (oc, s_effs, e_effs)
+    return (oc, s_conds, e_conds)
   }"
 
 definition 
-  "pddl_timed_effect \<equiv> do {
-    annotations \<leftarrow> (
-        ((pddl_keyword ''at'' -- pddl_keyword ''start'') *-- (return At_Start))
-      \<parallel> ((pddl_keyword ''at''-- pddl_keyword ''end'') *-- (return At_End))
-      ) <+? (\<lambda>x. shows ''Expected ground effect'' o x);
-    effects \<leftarrow> (
-      pddl_opt_and pddl_add_or_del
-      with (\<lambda>xs. (collect left_sum xs, collect right_sum xs)));
-    return (annotations, effects)
-  }"
-
-
-definition
-  "pddl_effects \<equiv> do {
-    effects \<leftarrow> pddl_keyword '':effects'' *-- pddl_opt_and pddl_timed_effect;
-    let combine_list_prod = (\<lambda>(a, b) (c, d). (a @ c, b @ c));
-    let combine_effects = (\<lambda>xs. 
-      fold combine_list_prod xs ([], [])
-      );
-    let start_effs = effects |> collect start_filter |> combine_effects;
-    let end_effs = effects |> collect end_filter |> combine_effects;
-    return (start_effs, end_effs)
+  "pddl_timed_effects \<equiv> do {
+    effs \<leftarrow> pddl_keyword '':effect'' *-- pddl_opt_and (pddl_timed_literal pddl_add_or_del);
+    let oc = effs |> collect oa_filter |> (\<lambda>xs. fold (@) xs []);
+    _ \<leftarrow> if (oc \<noteq> []) then error (shows ''\"over all\" effects not permitted'') else return ();
+  
+    let s_effs = effs |> collect start_filter |> (\<lambda>xs. fold (@) xs []);
+    let s_adds = s_effs |> collect add_filter;
+    let s_dels =  s_effs |> collect del_filter;
+    
+    let e_effs = effs |> collect end_filter |> (\<lambda>xs. fold (@) xs []);
+    let e_adds = e_effs |> collect add_filter;
+    let e_dels =  e_effs |> collect del_filter;
+    
+    return ((s_adds, s_dels), (e_adds, e_dels))
   }"
 
 definition
@@ -214,7 +236,7 @@ definition
    -- (pddl_action_params 
     *-- pddl_duration_constraints
      -- pddl_conditions
-     -- pddl_effects
+     -- pddl_timed_effects
       )
     ) with flat232"
 
@@ -229,21 +251,20 @@ definition
 
 definition
   "pddl_problem_head \<equiv> 
-    parens (
       parens (pddl_keyword ''problem'' *-- pddl_identifier)
-   -- pddl_domain_head)"
+   -- parens (pddl_keyword '':domain'' *-- pddl_identifier)"
 
 definition
   "pddl_init \<equiv>
     parens (
       pddl_keyword '':init'' 
-  *-- repeat (opt_parens pddl_predicate))"
+  *-- repeat1 pddl_predicate)"
 
 definition
   "pddl_goal \<equiv>
     parens (
       pddl_keyword '':goal''
-  *-- repeat (opt_parens pddl_predicate))"
+  *-- pddl_opt_and pddl_predicate)"
 
 
 definition
@@ -258,8 +279,35 @@ definition parse where
   "parse parser s \<equiv> case parse_all lx_ws parser s of
     Inl e \<Rightarrow> Error [e () ''Parser: '' |> String.implode]
   | Inr r \<Rightarrow> Result r"
+(* 
+value "parse (token (pddl_keyword ''domain'')) (STR '' domain'')"
 
 value [code] "parse pddl_goal (STR ''1234'')"
+
+value "parse pddl_num (STR ''123'')"
+
+value "parse (pddl_action_params -- pddl_duration_constraints) (STR '':parameters () :duration (and (>= ?duration 4)  (<= ?duration 4))'')"
+
+value "parse pddl_duration_constraint (STR ''(<= ?duration 4)'')"
+
+value "parse (pddl_opt_and pddl_duration_constraint) (STR ''(and (>= ?duration 4)  (<= ?duration 4))'')"
+
+value "parse pddl_duration_constraints (STR '':duration (and (>= ?duration 4)  (<= ?duration 4))'')"
+
+value "parse (pddl_keyword ''<='' with (\<lambda>_. duration_op.LEQ)) (STR ''<='')"
+
+value "parse pddl_init (STR ''(:init
+ (elevator-on-floor_e0_f2)
+ (stopped_e0)
+ (person-on-floor_p0_f0)
+)'')"
+
+value "parse pddl_goal (STR ''(:goal
+(and
+ (person-on-floor_p0_f1)
+ (person-on-floor_p0_f2)
+)
+)'')" *)
 
 ML_val \<open>
   @{code parse} @{code pddl_duration_constraints} "1234";\<close>
@@ -273,9 +321,21 @@ definition
   }"
 
 
+(* ML_val \<open>@{code parse} @{code pddl_domain_head} "(domain fasdf)"\<close>
+
+ML_val \<open>@{code parse} @{code pddl_requirements} "(:requirements :strips)"\<close>
+
+ML_val \<open>@{code parse} @{code pddl_problem_head} "(problem groundproblem) (:domain ground)"\<close>
+
+ML_val \<open>@{code parse} @{code pddl_predicates} "(:predicates (elevator-on-floor_e0_f2))"\<close>
+
+ML_val \<open>@{code parse} @{code pddl_durative_action} 
+"(:durative-action _enter-elevator_p0_e0_f0_ :parameters () :duration (and (>= ?duration 4)  (<= ?duration 4)) :condition(and (over all (elevator-on-floor_e0_f0)) (over all (stopped_e0))(at start (person-on-floor_p0_f0)) ) :effect (and (at start (not (person-on-floor_p0_f0)))(at end (person-in-elevator_p0_e0)) ))"\<close>
+
+ *)
 
 ML \<open>
-  fun parse_domain_and_prob df pf =
+  fun parse_domain_and_problem df pf =
   let 
     val p = file_to_string pf; 
     val d = file_to_string df
@@ -284,6 +344,12 @@ ML \<open>
   end
 \<close>
 
+(* ML_val \<open>OS.FileSys.getDir()\<close>
 
+ML_val \<open>
+  parse_domain_and_problem
+  "work/temporal_planning_certification/temporal-planning-certification/examples/ground-elevators.pddl"
+  "work/temporal_planning_certification/temporal-planning-certification/examples/ground-elevators-prob1.pddl"
+\<close> *)
 
 end
