TA_Network/TP_NTA_Printing.thy
@@ -1,0 +1,5 @@
+theory TP_NTA_Printing
+imports TP_NTA_Reduction
+begin
+
+end
